theories/link.v
@@ -10,7 +10,7 @@ Set Default Proof Using "Type".
 
 Section mod_link.
   Context {EV : Type} {S : Type}.
-  Implicit Types (R : seq_product_state → S → EV → seq_product_state → S → EV → Prop).
+  Implicit Types (R : seq_product_state → S → EV → seq_product_state → S → EV → bool → Prop).
   Implicit Types (m : module (io_event EV)).
 
 (*
@@ -78,34 +78,38 @@ Section mod_link.
 *)
   Inductive mod_link_state :=
   | MLFLeft | MLFRight | MLFNone
-  | MLFRecvL (e : EV) | MLFRecvR (e : EV).
+  | MLFRecvL (e : EV) | MLFRecvR (e : EV)
+  | MLFUb (sp : seq_product_state).
 
-  Definition mod_link_to_state (s : seq_product_state) (e : EV) : mod_link_state :=
-    match s with
-    | SPNone => MLFNone
-    | SPLeft => MLFRecvL e
-    | SPRight => MLFRecvR e
-    end.
+  Definition mod_link_to_state (ok : bool) (s : seq_product_state) (e : EV) : mod_link_state :=
+    if ok then
+      match s with
+      | SPNone => MLFNone
+      | SPLeft => MLFRecvL e
+      | SPRight => MLFRecvR e
+      end
+    else
+      MLFUb s.
   Inductive mod_link_filter R : mod_map_fn (seq_product_event (io_event EV) (io_event EV)) (io_event EV) (mod_link_state * S) :=
-  | MLFLeftS s e p' s' e':
-    R SPLeft s e p' s' e' →
+  | MLFLeftS s e p' s' e' ok:
+    R SPLeft s e p' s' e' ok →
     mod_link_filter R (MLFLeft, s) (SPELeft (Outgoing, e) p')
                     (if p' is SPNone then Some (Outgoing, e') else None)
-                    (mod_link_to_state p' e', s')
+                    (mod_link_to_state ok p' e', s') ok
   | MLFLeftRecvS s e:
-    mod_link_filter R (MLFRecvL e, s) (SPELeft (Incoming, e) SPLeft) None (MLFLeft, s)
-  | MLFRightS s e p' s' e':
-    R SPRight s e p' s' e' →
+    mod_link_filter R (MLFRecvL e, s) (SPELeft (Incoming, e) SPLeft) None (MLFLeft, s) true
+  | MLFRightS s e p' s' e' ok:
+    R SPRight s e p' s' e' ok →
     mod_link_filter R (MLFRight, s) (SPERight (Outgoing, e) p')
                     (if p' is SPNone then Some (Outgoing, e') else None)
-                    (mod_link_to_state p' e', s')
+                    (mod_link_to_state ok p' e', s') ok
   | MLFRightRecvS s e:
-    mod_link_filter R (MLFRecvR e, s) (SPERight (Incoming, e) SPRight) None (MLFRight, s)
-  | MLFNoneS s e p' s' e':
-    R SPNone s e p' s' e' →
+    mod_link_filter R (MLFRecvR e, s) (SPERight (Incoming, e) SPRight) None (MLFRight, s) true
+  | MLFNoneS s e p' s' e' ok:
+    R SPNone s e p' s' e' ok →
     mod_link_filter R (MLFNone, s) (SPENone p')
                     (Some (Incoming, e'))
-                    (mod_link_to_state p' e', s')
+                    (mod_link_to_state ok p' e', s') ok
   .
 
   Definition mod_link_trans R m1 m2 (σ : mod_link_state * S * m1.(m_state) * m2.(m_state)) :=
@@ -113,7 +117,8 @@ Section mod_link.
           | MLFLeft | MLFRecvL _ => SPLeft
           | MLFRight | MLFRecvR _ => SPRight
           | MLFNone => SPNone
-          end, σ.1.2, σ.2, σ.1.1).
+          | MLFUb sp => sp
+          end, σ.1.2, σ.2, (σ.1.1, if σ.1.1.1 is MLFUb _ then false else true)).
   Arguments mod_link_trans _ _ _ _ /.
 
   Definition mod_link R m1 m2 : module (io_event EV) :=
@@ -124,11 +129,11 @@ Section mod_link.
     VisNoAll (mod_link R m1 m2).
   Proof.
     apply: mod_state_transform_vis_no_all.
-    move => ??? [[[sp σ1]σ2][σ s]] ?.
+    move => ??? [[[sp σ1]σ2][[σ s] ok]] ??.
     eexists (σ, s, σ1, σ2) => -[[[??]?]?]/=.
     split => ?; simplify_eq => //.
     invert_all @m_step; invert_all @mod_link_filter; destruct_all?; simplify_eq.
-    all: unfold mod_link_to_state in *; repeat case_match => //; by simplify_eq.
+    all: unfold mod_link_to_state in *; repeat case_match => //; simplify_eq => //.
   Qed.
 
   Lemma mod_link_trefines R m1 m2 m1' m2' σ1 σ2 σ1' σ2' σ `{!VisNoAll m1} `{!VisNoAll m2}:
@@ -139,10 +144,10 @@ Section mod_link.
     move => ??.
     apply: mod_state_transform_trefines; [| | |done..].
     - move => [[??]?] [[[??]?]?] [[[??]?]?] /=. naive_solver.
-    - move => [[??]?] [[[??]?][??]] [[[??]?][??]] ?????; simplify_eq.
+    - move => [[??]?] [[[??]?][[??]?]] [[[??]?][[??]?]] ?????; simplify_eq.
       invert_all @m_step; invert_all @mod_link_filter; destruct_all?; simplify_eq.
       all: eexists (_, _, _); do 3 f_equal; repeat case_match => //; simplify_eq/= => //.
-      all: unfold mod_link_to_state in *; by repeat case_match.
+      all: unfold mod_link_to_state in *; repeat case_match; simplify_eq => //.
     - apply mod_map_trefines => /=. by apply mod_seq_product_trefines.
   Qed.
 
@@ -150,9 +155,9 @@ Section mod_link.
     TStepI (mod_link R m1 m2) (MLFLeft, s, σ1, σ2) (λ G, P (λ b κ P',
       match κ with
       | None => G b None (λ G', P' (λ x, G' (MLFLeft, s, x, σ2)))
-      | Some κ' => ∀ p' s' e', R SPLeft s κ'.2 p' s' e' → κ'.1 = Outgoing →
+      | Some κ' => ∀ p' s' e' ok, R SPLeft s κ'.2 p' s' e' ok → κ'.1 = Outgoing →
                               G b (if p' is SPNone then Some (Outgoing, e') else None)
-                               (λ G', P' (λ x, G' (mod_link_to_state p' e', s', x, σ2)))
+                               (λ G', P' (λ x, G' (mod_link_to_state ok p' e', s', x, σ2)))
       end)).
   Proof.
     constructor => G /tstepi_proof?. clear TStepI0.
@@ -163,16 +168,16 @@ Section mod_link.
       + case_match; simplify_eq. invert_all @mod_link_filter.
         split!; [done| |done] => /=?. destruct_all?.
         split!; [naive_solver..|]. move => /= ? HP. move: HP => /H2[?[??]]. eexists (_, _, _, _).
-        split!; [|done|naive_solver] => /=. by destruct s0.
+        split!; [by destruct ok, s0|done|by destruct ok, s0|naive_solver].
   Qed.
 
   Lemma mod_link_step_right_i R m1 m2 s σ1 σ2 P `{!TStepI m2 σ2 P} :
     TStepI (mod_link R m1 m2) (MLFRight, s, σ1, σ2) (λ G, P (λ b κ P',
       match κ with
       | None => G b None (λ G', P' (λ x, G' (MLFRight, s, σ1, x)))
-      | Some κ' => ∀ p' s' e', R SPRight s κ'.2 p' s' e' → κ'.1 = Outgoing →
+      | Some κ' => ∀ p' s' e' ok, R SPRight s κ'.2 p' s' e' ok → κ'.1 = Outgoing →
                               G b (if p' is SPNone then Some (Outgoing, e') else None)
-                               (λ G', P' (λ x, G' (mod_link_to_state p' e', s', σ1, x)))
+                               (λ G', P' (λ x, G' (mod_link_to_state ok p' e', s', σ1, x)))
       end)).
   Proof.
     constructor => G /tstepi_proof?. clear TStepI0.
@@ -183,7 +188,7 @@ Section mod_link.
       + case_match; simplify_eq. invert_all @mod_link_filter.
         split!; [done| |done] => /=?. destruct_all?.
         split!; [naive_solver..|]. move => /= ? HP. move: HP => /H2[?[??]]. eexists (_, _, _, _).
-        split!; [|done|naive_solver] => /=. by destruct s0.
+        split!; [by destruct s0, ok|done|by destruct s0, ok|naive_solver] => /=.
   Qed.
 
   Lemma mod_link_step_left_recv_i R m1 m2 s σ1 σ2 e P `{!TStepI m1 σ1 P} :
@@ -217,21 +222,21 @@ Section mod_link.
   Qed.
 
   Lemma mod_link_step_none_i R m1 m2 s σ1 σ2 :
-    TStepI (mod_link R m1 m2) (MLFNone, s, σ1, σ2) (λ G, ∀ e p' s' e', R SPNone s e p' s' e' →
-      G true (Some (Incoming, e')) (λ G', G' (mod_link_to_state p' e', s', σ1, σ2))).
+    TStepI (mod_link R m1 m2) (MLFNone, s, σ1, σ2) (λ G, ∀ e p' s' e' ok, R SPNone s e p' s' e' ok →
+      G true (Some (Incoming, e')) (λ G', G' (mod_link_to_state ok p' e', s', σ1, σ2))).
   Proof.
     constructor => G HG. apply steps_impl_step_end => ???.
     invert_all' @m_step; simplify_eq/=; invert_all' mod_link_filter; simplify_eq/=.
-    split!; [naive_solver|done|] => /= ??. eexists (_, _, _, _). split!. by destruct s0.
+    split!; [naive_solver|done|] => /= ??. eexists (_, _, _, _). split!; by destruct s0, ok.
   Qed.
 
   Lemma mod_link_step_left_s R m1 m2 s σ1 σ2 P `{!TStepS m1 σ1 P} :
     TStepS (mod_link R m1 m2) (MLFLeft, s, σ1, σ2) (λ G, P (λ κ P',
       match κ with
       | None => G None (λ G', P' (λ x, G' (MLFLeft, s, x, σ2)))
-      | Some (Outgoing, e) => ∃ p' s' e', R SPLeft s e p' s' e' ∧
+      | Some (Outgoing, e) => ∃ p' s' e' ok, R SPLeft s e p' s' e' ok ∧
                               G (if p' is SPNone then Some (Outgoing, e') else None)
-                               (λ G', P' (λ σ', G' (mod_link_to_state p' e', s', σ', σ2)))
+                               (λ G', P' (λ σ', G' (mod_link_to_state ok p' e', s', σ', σ2)))
       | Some _ => False
       end)).
   Proof.
@@ -246,9 +251,9 @@ Section mod_link.
     TStepS (mod_link R m1 m2) (MLFRight, s, σ1, σ2) (λ G, P (λ κ P',
       match κ with
       | None => G None (λ G', P' (λ x, G' (MLFRight, s, σ1, x)))
-      | Some (Outgoing, e) => ∃ p' s' e', R SPRight s e p' s' e' ∧
+      | Some (Outgoing, e) => ∃ p' s' e' ok, R SPRight s e p' s' e' ok ∧
                               G (if p' is SPNone then Some (Outgoing, e') else None)
-                               (λ G', P' (λ σ', G' (mod_link_to_state p' e', s', σ1, σ')))
+                               (λ G', P' (λ σ', G' (mod_link_to_state ok p' e', s', σ1, σ')))
       | Some _ => False
       end)).
   Proof.
@@ -290,13 +295,17 @@ Section mod_link.
   Qed.
 
   Lemma mod_link_step_none_s R m1 m2 s σ1 σ2 :
-    TStepS (mod_link R m1 m2) (MLFNone, s, σ1, σ2) (λ G, ∃ e p' s' e', R SPNone s e p' s' e' ∧
-      G (Some (Incoming, e')) (λ G', G' (mod_link_to_state p' e', s', σ1, σ2))).
+    TStepS (mod_link R m1 m2) (MLFNone, s, σ1, σ2) (λ G, ∃ e p' s' e' ok, R SPNone s e p' s' e' ok ∧
+      G (Some (Incoming, e')) (λ G', G' (mod_link_to_state ok p' e', s', σ1, σ2))).
   Proof.
-    constructor => G [?[?[?[?[??]]]]]. split!; [done|] => /=??.
+    constructor => G [?[?[?[?[?[??]]]]]]. split!; [done|] => /=??.
     tstep_s. split!; [by econs|]. move => [[[??]?]?] /=. unfold mod_link_to_state.
     repeat case_match; naive_solver.
   Qed.
+
+  Lemma mod_link_step_ub_s R m1 m2 s σ1 σ2 sp :
+    TStepS (mod_link R m1 m2) (MLFUb sp, s, σ1, σ2) (λ G, G None (λ G', True)).
+  Proof. constructor => G ?. split!; [done|] => /=??. by tstep_s. Qed.
 End mod_link.
 Arguments mod_link_trans _ _ _ _ _ /.
 Arguments mod_link_state : clear implicits.
@@ -312,4 +321,5 @@ Global Hint Resolve
        mod_link_step_left_recv_s
        mod_link_step_right_recv_s
        mod_link_step_none_s
+       mod_link_step_ub_s
 | 2 : tstep.
